Remove runtime_scope
As per https://github.com/mit-plv/fiat-crypto/pull/315#discussion_r169085799

src/Experiments/SimplyTypedArithmetic.v
@@ -18,14 +18,6 @@ Require Import Crypto.Util.ZUtil.Tactics.LtbToLt.
 Require Import Crypto.Util.Notations.
 Import ListNotations. Local Open Scope Z_scope.
 
-Definition runtime_mul := Z.mul.
-Definition runtime_add := Z.add.
-Definition runtime_opp := Z.opp.
-Delimit Scope runtime_scope with RT.
-Infix "*" := runtime_mul : runtime_scope.
-Infix "+" := runtime_add : runtime_scope.
-Notation "- a" := (runtime_opp a%RT) : runtime_scope.
-
 Module Associational.
   Definition eval (p:list (Z*Z)) : Z :=
     fold_right Z.add 0%Z (map (fun t => fst t * snd t) p).
@@ -51,14 +43,14 @@ Module Associational.
   Definition mul (p q:list (Z*Z)) : list (Z*Z) :=
     flat_map (fun t =>
       map (fun t' =>
-        (fst t * fst t', (snd t * snd t')%RT))
+        (fst t * fst t', snd t * snd t'))
     q) p.
   Lemma eval_mul p q : eval (mul p q) = eval p * eval q.
   Proof. induction p; cbv [mul]; push; nsatz.                 Qed.
   Hint Rewrite eval_mul : push_eval.
 
   Definition negate_snd (p:list (Z*Z)) : list (Z*Z) :=
-    map (fun cx => (fst cx, (-snd cx)%RT)) p.
+    map (fun cx => (fst cx, -snd cx)) p.
   Lemma eval_negate_snd p : eval (negate_snd p) = - eval p.
   Proof. induction p; cbv [negate_snd]; push; nsatz.          Qed.
   Hint Rewrite eval_negate_snd : push_eval.
@@ -69,7 +61,7 @@ Module Associational.
     (* Goal: eval ?ab = eval [(10,a1);(1,a0)] * eval [(10,b1);(1,b0)] *)
     rewrite <-eval_mul.
     (* Goal: eval ?ab = eval (mul [(10,a1);(1,a0)] [(10,b1);(1,b0)]) *)
-    cbv -[runtime_mul eval].
+    cbv -[Z.mul eval]; cbn -[eval].
     (* Goal: eval ?ab = eval [(100,(a1*b1));(10,a1*b0);(10,a0*b1);(1,a0*b0)]%RT *)
     trivial.                                              Defined.
 
@@ -153,13 +145,13 @@ Module Positional. Section Positional.
     generalize dependent (List.seq 0 n); intro xs.
     induction xs; simpl; nsatz.                               Qed.
   Definition add_to_nth i x (ls : list Z) : list Z
-    := ListUtil.update_nth i (fun y => runtime_add x y) ls.
+    := ListUtil.update_nth i (fun y => x + y) ls.
   Lemma eval_add_to_nth (n:nat) (i:nat) (x:Z) (xs:list Z) (H:(i<length xs)%nat)
         (Hn : length xs = n) (* N.B. We really only need [i < Nat.min n (length xs)] *) :
     eval n (add_to_nth i x xs) = weight i * x + eval n xs.
   Proof.
     subst n.
-    cbv [eval to_associational add_to_nth runtime_add].
+    cbv [eval to_associational add_to_nth].
     rewrite ListUtil.combine_update_nth_r at 1.
     rewrite <-(update_nth_id i (List.combine _ _)) at 2.
     rewrite <-!(ListUtil.splice_nth_equiv_update_nth_update _ _
@@ -175,11 +167,11 @@ Module Positional. Section Positional.
   Definition place (t:Z*Z) (i:nat) : nat * Z :=
     nat_rect
       (fun _ => (nat * Z)%type)
-      ((O, fst t * snd t)%RT)
+      (O, fst t * snd t)
       (fun i' place_i'
        => let i := S i' in
           if (fst t mod weight i =? 0)
-          then (i, let c := fst t / weight i in (c * snd t)%RT)
+          then (i, let c := fst t / weight i in c * snd t)
           else place_i')
       i.
 
@@ -772,8 +764,6 @@ Module Compilers.
           | List_fold_right {A B} : ident ((B * A -> A) * A * list B) A
           | List_update_nth {T} : ident (nat * (T -> T) * list T) (list T)
           | List_nth_default {T} : ident (T * list T * nat) T
-          | Z_runtime_mul : ident (Z * Z) Z
-          | Z_runtime_add : ident (Z * Z) Z
           | Z_add : ident (Z * Z) Z
           | Z_mul : ident (Z * Z) Z
           | Z_pow : ident (Z * Z) Z
@@ -819,8 +809,6 @@ Module Compilers.
                | List_fold_right A B => curry3_1 (@List.fold_right (type.interp A) (type.interp B))
                | List_update_nth T => curry3 (@update_nth (type.interp T))
                | List_nth_default T => curry3 (@List.nth_default (type.interp T))
-               | Z_runtime_mul => curry2 runtime_mul
-               | Z_runtime_add => curry2 runtime_add
                | Z_add => curry2 Z.add
                | Z_mul => curry2 Z.mul
                | Z_pow => curry2 Z.pow
@@ -914,8 +902,6 @@ Module Compilers.
             | @List.nth_default ?T ?d ?ls ?n
               => let rT := type.reify T in
                  mkAppIdent (@ident.List_nth_default rT) (d, ls, n)
-            | runtime_mul ?x ?y => mkAppIdent ident.Z_runtime_mul (x, y)
-            | runtime_add ?x ?y => mkAppIdent ident.Z_runtime_add (x, y)
             | Z.add ?x ?y => mkAppIdent ident.Z_add (x, y)
             | Z.mul ?x ?y => mkAppIdent ident.Z_mul (x, y)
             | Z.pow ?x ?y => mkAppIdent ident.Z_pow (x, y)
@@ -953,8 +939,6 @@ Module Compilers.
           End List.
 
           Module Z.
-            Notation runtime_mul := Z_runtime_mul.
-            Notation runtime_add := Z_runtime_add.
             Notation add := Z_add.
             Notation mul := Z_mul.
             Notation pow := Z_pow.
@@ -1018,10 +1002,8 @@ Module Compilers.
           | list_rect {A P} : ident (P * (A * list A * P -> P) * list A) P
           | List_nth_default {T} : ident (T * list T * nat) T
           | List_nth_default_concrete {T : type.primitive} (d : interp T) (n : Datatypes.nat) : ident (list T) T
-          | Z_runtime_mul : ident (Z * Z) Z
-          | Z_runtime_add : ident (Z * Z) Z
-          | Z_runtime_shiftr (offset : BinInt.Z) : ident Z Z
-          | Z_runtime_land (mask : BinInt.Z) : ident Z Z
+          | Z_shiftr (offset : BinInt.Z) : ident Z Z
+          | Z_land (mask : BinInt.Z) : ident Z Z
           | Z_add : ident (Z * Z) Z
           | Z_mul : ident (Z * Z) Z
           | Z_pow : ident (Z * Z) Z
@@ -1061,10 +1043,8 @@ Module Compilers.
                | list_rect A P => curry3_23 (@Datatypes.list_rect (type.interp A) (fun _ => type.interp P))
                | List_nth_default T => curry3 (@List.nth_default (type.interp T))
                | List_nth_default_concrete T d n => fun ls => @List.nth_default (type.interp T) d ls n
-               | Z_runtime_mul => curry2 runtime_mul
-               | Z_runtime_add => curry2 runtime_add
-               | Z_runtime_shiftr n => fun v => Z.shiftr v n
-               | Z_runtime_land mask => fun v => Z.land v mask
+               | Z_shiftr n => fun v => Z.shiftr v n
+               | Z_land mask => fun v => Z.land v mask
                | Z_add => curry2 Z.add
                | Z_mul => curry2 Z.mul
                | Z_pow => curry2 Z.pow
@@ -1137,8 +1117,6 @@ Module Compilers.
             | @List.nth_default ?T ?d ?ls ?n
               => let rT := type.reify T in
                  mkAppIdent (@ident.List_nth_default rT) (d, ls, n)
-            | runtime_mul ?x ?y => mkAppIdent ident.Z_runtime_mul (x, y)
-            | runtime_add ?x ?y => mkAppIdent ident.Z_runtime_add (x, y)
             | Z.add ?x ?y => mkAppIdent ident.Z_add (x, y)
             | Z.mul ?x ?y => mkAppIdent ident.Z_mul (x, y)
             | Z.pow ?x ?y => mkAppIdent ident.Z_pow (x, y)
@@ -1167,10 +1145,8 @@ Module Compilers.
           End List.
 
           Module Z.
-            Notation runtime_mul := Z_runtime_mul.
-            Notation runtime_add := Z_runtime_add.
-            Notation runtime_shiftr := Z_runtime_shiftr.
-            Notation runtime_land := Z_runtime_land.
+            Notation shiftr := Z_shiftr.
+            Notation land := Z_land.
             Notation add := Z_add.
             Notation mul := Z_mul.
             Notation pow := Z_pow.
@@ -1258,10 +1234,6 @@ Module Compilers.
                => AppIdent ident.pred
              | for_reification.ident.primitive t v
                => AppIdent (ident.primitive v)
-             | for_reification.ident.Z_runtime_mul
-               => AppIdent ident.Z.runtime_mul
-             | for_reification.ident.Z_runtime_add
-               => AppIdent ident.Z.runtime_add
              | for_reification.ident.Z_add
                => AppIdent ident.Z.add
              | for_reification.ident.Z_mul
@@ -2029,10 +2001,8 @@ Module Compilers.
                   | ident.primitive _ _ as idc
                   | ident.Nat_succ as idc
                   | ident.pred as idc
-                  | ident.Z_runtime_mul as idc
-                  | ident.Z_runtime_add as idc
-                  | ident.Z_runtime_shiftr _ as idc
-                  | ident.Z_runtime_land _ as idc
+                  | ident.Z_shiftr _ as idc
+                  | ident.Z_land _ as idc
                   | ident.Z_add as idc
                   | ident.Z_mul as idc
                   | ident.Z_pow as idc
@@ -2198,16 +2168,14 @@ Module Compilers.
                      (ident.snd @@ (Var xyk))
                        @ ((idc : default.ident _ type.nat)
                             @@ (ident.fst @@ (Var xyk)))
-                | ident.Z_runtime_shiftr _ as idc
-                | ident.Z_runtime_land _ as idc
+                | ident.Z_shiftr _ as idc
+                | ident.Z_land _ as idc
                 | ident.Z_opp as idc
                   => λ (xyk :
                           (* ignore this line; it's to work around lack of fixpoint refolding in type inference *) var (type.Z * (type.Z -> R))%ctype) ,
                      (ident.snd @@ (Var xyk))
                        @ ((idc : default.ident _ type.Z)
                             @@ (ident.fst @@ (Var xyk)))
-                | ident.Z_runtime_mul as idc
-                | ident.Z_runtime_add as idc
                 | ident.Z_add as idc
                 | ident.Z_mul as idc
                 | ident.Z_pow as idc
@@ -2817,15 +2785,13 @@ Module Compilers.
              | ident.Nat_succ as idc
              | ident.Z_of_nat as idc
              | ident.Z_opp as idc
-             | ident.Z_runtime_shiftr _ as idc
-             | ident.Z_runtime_land _ as idc
+             | ident.Z_shiftr _ as idc
+             | ident.Z_land _ as idc
                => fun x : expr _ + type.interp _
                   => match x return expr _ + type.interp _ with
                      | inr x => inr (ident.interp idc x)
                      | inl x => expr.reflect (AppIdent idc x)
                      end
-             | ident.Z_add as idc
-             | ident.Z_mul as idc
              | ident.Z_pow as idc
              | ident.Z_eqb as idc
                => fun (x_y : expr (_ * _) + (expr _ + type.interp _) * (expr _ + type.interp _))
@@ -2840,7 +2806,7 @@ Module Compilers.
                      | inr (inr x, inr y) => inr (ident.interp idc (x, y))
                      | inr (x, inr y)
                        => if Z.eqb y (2^Z.log2 y)
-                          then expr.reflect (AppIdent (ident.Z.runtime_shiftr (Z.log2 y)) (expr.reify (t:=type.Z) x))
+                          then expr.reflect (AppIdent (ident.Z.shiftr (Z.log2 y)) (expr.reify (t:=type.Z) x))
                           else default
                      | _ => default
                      end
@@ -2851,11 +2817,11 @@ Module Compilers.
                      | inr (inr x, inr y) => inr (ident.interp idc (x, y))
                      | inr (x, inr y)
                        => if Z.eqb y (2^Z.log2 y)
-                          then expr.reflect (AppIdent (ident.Z.runtime_land (y-1)) (expr.reify (t:=type.Z) x))
+                          then expr.reflect (AppIdent (ident.Z.land (y-1)) (expr.reify (t:=type.Z) x))
                           else default
                      | _ => default
                      end
-             | ident.Z_runtime_mul as idc
+             | ident.Z_mul as idc
                => fun (x_y : expr (_ * _) + (expr _ + type.interp _) * (expr _ + type.interp _))
                   => let default := expr.reflect (AppIdent idc (expr.reify (t:=_*_) x_y)) in
                      match x_y return expr _ + type.interp _ with
@@ -2869,7 +2835,7 @@ Module Compilers.
                                else default
                      | inr (inl _, inl _) | inl _ => default
                      end
-             | ident.Z_runtime_add as idc
+             | ident.Z_add as idc
                => fun (x_y : expr (_ * _) + (expr _ + type.interp _) * (expr _ + type.interp _))
                   => let default := expr.reflect (AppIdent idc (expr.reify (t:=_*_) x_y)) in
                      match x_y return expr _ + type.interp _ with
@@ -2916,7 +2882,6 @@ Module Compilers.
 
       Fixpoint to_mul_list (e : @expr var type.Z) : list (@expr var type.Z)
         := match e in expr.expr t return list (@expr var t) with
-           | AppIdent s type.Z ident.Z_runtime_mul (Pair type.Z type.Z x y)
            | AppIdent s type.Z ident.Z_mul (Pair type.Z type.Z x y)
              => to_mul_list x ++ to_mul_list y
            | Var _ _ as e
@@ -2930,10 +2895,8 @@ Module Compilers.
 
       Fixpoint to_add_mul_list (e : @expr var type.Z) : list (list (@expr var type.Z))
         := match e in expr.expr t return list (list (@expr var t)) with
-           | AppIdent s type.Z ident.Z_runtime_add (Pair type.Z type.Z x y)
            | AppIdent s type.Z ident.Z_add (Pair type.Z type.Z x y)
              => to_add_mul_list x ++ to_add_mul_list y
-           | AppIdent s type.Z ident.Z_runtime_mul (Pair type.Z type.Z x y)
            | AppIdent s type.Z ident.Z_mul (Pair type.Z type.Z x y)
              => [to_mul_list x ++ to_mul_list y]
            | Var _ _ as e
@@ -3369,15 +3332,13 @@ Module Compilers.
                | default.ident.List_nth_default T => None
                | ident.List_nth_default_concrete T d n
                  => Some (@List_nth (type.primitive.compile T) n)
-               | ident.Z_runtime_mul
                | default.ident.Z_mul
                  => Some Z.mul
-               | ident.Z_runtime_add
                | default.ident.Z_add
                  => Some Z.add
-               | ident.Z_runtime_shiftr n
+               | ident.Z_shiftr n
                  => Some (Z.shiftr n)
-               | ident.Z_runtime_land mask
+               | ident.Z_land mask
                  => Some (Z.land mask)
                | ident.Z_pow
                | ident.Z_opp
@@ -3835,25 +3796,17 @@ Local Coercion QArith_base.inject_Z : Z >-> Q.
 - reassociation
 - indexed + bounds analysis + of phoas *)
 
-Delimit Scope RT_expr_scope with RT_expr.
 Import Uncurried.
 Import expr.
 Import for_reification.Notations.Reification.
 
 Notation "x + y"
-  := (AppIdent ident.Z.runtime_add (x%RT_expr, y%RT_expr)%expr)
-     : RT_expr_scope.
-Notation "x * y"
-  := (AppIdent ident.Z.runtime_mul (x%RT_expr, y%RT_expr)%expr)
-     : RT_expr_scope.
-Notation "x + y"
-  := (AppIdent ident.Z.runtime_add (x%RT_expr, y%RT_expr)%expr)
+  := (AppIdent ident.Z.add (x, y)%expr)
      : expr_scope.
 Notation "x * y"
-  := (AppIdent ident.Z.runtime_mul (x%RT_expr, y%RT_expr)%expr)
+  := (AppIdent ident.Z.mul (x, y)%expr)
      : expr_scope.
 Notation "x" := (Var x) (only printing, at level 9) : expr_scope.
-Open Scope RT_expr_scope.
 
 Require Import AdmitAxiom.
 
@@ -3874,8 +3827,8 @@ Module test2.
   Proof.
     let v := Reify (fun y : Z
                     => (fun k : Z * Z -> Z * Z
-                        => dlet_nd x := (y * y)%RT in
-                            dlet_nd z := (x * x)%RT in
+                        => dlet_nd x := (y * y) in
+                            dlet_nd z := (x * x) in
                             k (z, z))
                          (fun v => v)) in
     pose v as E.
@@ -3885,8 +3838,8 @@ Module test2.
     lazymatch (eval cbv delta [E'] in E') with
     | (fun var : type -> Type =>
          (λ x : var (type.type_primitive type.Z),
-                expr_let x0 := (Var x * Var x)%RT_expr in
-              expr_let x1 := (Var x0 * Var x0)%RT_expr in
+                expr_let x0 := (Var x * Var x) in
+              expr_let x1 := (Var x0 * Var x0) in
               (Var x1, Var x1))%expr) => idtac
     end.
     Import BoundsAnalysis.ident.
@@ -3909,11 +3862,11 @@ Module test3.
   Example test3 : True.
   Proof.
     let v := Reify (fun y : Z
-                    => dlet_nd x := dlet_nd x := (y * y)%RT in
-                        (x * x)%RT in
-                        dlet_nd z := dlet_nd z := (x * x)%RT in
-                        (z * z)%RT in
-                        (z * z)%RT) in
+                    => dlet_nd x := dlet_nd x := (y * y) in
+                        (x * x) in
+                        dlet_nd z := dlet_nd z := (x * x) in
+                        (z * z) in
+                        (z * z)) in
     pose v as E.
     vm_compute in E.
     pose (PartialReduce (CPS.CallFunWithIdContinuation (CPS.Translate (canonicalize_list_recursion E)))) as E'.
@@ -3925,7 +3878,7 @@ Module test3.
               expr_let x1 := Var x0 * Var x0 in
               expr_let x2 := Var x1 * Var x1 in
               expr_let x3 := Var x2 * Var x2 in
-              Var x3 * Var x3)%RT_expr%expr)
+              Var x3 * Var x3)%expr)
       => idtac
     end.
     Import BoundsAnalysis.ident.
@@ -3955,8 +3908,8 @@ Module test4.
     let v := Reify (fun y : (list Z * list Z)
                     => dlet_nd x := List.nth_default (-1) (fst y) 0 in
                         dlet_nd z := List.nth_default (-1) (snd y) 0 in
-                        dlet_nd xz := (x * z)%RT in
-                        (xz :: xz :: nil)%RT) in
+                        dlet_nd xz := (x * z) in
+                        (xz :: xz :: nil)) in
     pose v as E.
     vm_compute in E.
     pose (PartialReduce (CPS.CallFunWithIdContinuation (CPS.Translate (canonicalize_list_recursion E)))) as E'.
@@ -3986,7 +3939,7 @@ Module test5.
   Example test5 : True.
   Proof.
     let v := Reify (fun y : (Z * Z)
-                    => dlet_nd x := (13 * (fst y * snd y))%RT in
+                    => dlet_nd x := (13 * (fst y * snd y)) in
                         x) in
     pose v as E.
     vm_compute in E.
@@ -4010,7 +3963,7 @@ Module test6.
   Proof.
     let v := Reify (fun y : Z
                     => if 0 =? 1
-                       then dlet_nd x := (y * y)%RT in
+                       then dlet_nd x := (y * y) in
                                 x
                        else y) in
     pose v as E.
